theories/CTree/Logic/Trans.v
@@ -16,6 +16,8 @@ From CTree Require Import
   CTree.Core
   CTree.Pred
   CTree.Equ
+  CTree.SBisim
+  Utils.Trc
   CTree.Trans
   CTree.Events.Writer
   Events.Core
@@ -31,63 +33,88 @@ Notation ctreeEW E := (ctree (writerE (Bar E))).
 
 Section CTreeTrans.
   Context {E: Type} `{HE: Encode E} {X: Type}.
-  Notation opt E := (option (Bar E)).
 
-  Variant ktrans_: relation (ctree E X * opt E) :=    
-    | KtransObs (ts: opt E) (e: E) (x: encode e)
+  (* Note: This Kripke transition rel observes labels, this is important
+     for the [ktrans_bind_inv] lemma *)
+  Variant ktrans_: relation (ctree E X * World E) :=    
+    | KtransObs (ts: World E) (e: E) (x: encode e)
         (t t': ctree E X):
       trans (obs e x) t t' ->
-      ktrans_ (t, ts) (t', Some (Obs e x))
-    | KtransTau (ts: opt E) (t t': ctree E X):
+      ~ is_done ts ->
+      ktrans_ (t, ts) (t', Obs e x)
+    | KtransTau (ts: World E) (t t': ctree E X):
       trans tau t t' ->
-      ktrans_ (t, ts) (t', ts).
+      ~ is_done ts ->
+      ktrans_ (t, ts) (t', ts)
+    | KtransRet (ts: World E) (t t': ctree E X) (x: X):
+      trans (val x) t stuck ->
+      ~ is_done ts ->
+      t' ≅ stuck ->
+      ktrans_ (t, ts) (t', Done x).
 
-  (*| This version is more amenable to induction |*)
-  Lemma ktrans_trans: forall t t' w w',
-      ktrans_ (t, w) (t', w') <->
-        (exists l, trans_ l (observe t) (observe t') /\
-                ((l = tau /\ w' = w)
-                 \/ (exists e (x: encode e), l = obs e x /\ w' = Some (Obs e x)))).
-  Proof.
-    intros; split; intro H.
-    inv H. 
-    - exists (obs e x); split; auto.
-      right; exists e, x; auto.
-    - exists tau; split; auto.
-    - destruct H as (l & H & [(-> & ->) | (e & x & -> & ->)]). 
-      + now apply KtransTau.
-      + now apply KtransObs.
-  Qed.
-  
   Global Instance trans_equ_proper:
     Proper (equ eq * eq ==> equ eq * eq ==> iff) ktrans_.
   Proof.
     unfold Proper, respectful, RelCompFun, fst, snd;
       cbn; intros.
-    destruct2 H0; destruct2 H; destruct x, y, x0, y0; subst.
+    destruct2 H; destruct2 H0; destruct x, y, x0, y0; subst.
     split; intros TR; inv TR.
-    - apply KtransObs; now rewrite <- Heqt0, <- Heqt. 
-    - apply KtransTau; now rewrite <- Heqt0, <- Heqt.
-    - apply KtransObs; now rewrite Heqt0, Heqt.
-    - apply KtransTau; now rewrite Heqt0, Heqt.
+    - apply KtransObs; auto. now rewrite <- Heqt0, <- Heqt. 
+    - apply KtransTau; auto. now rewrite <- Heqt0, <- Heqt.
+    - apply KtransRet; auto.
+      + now rewrite <- Heqt.
+      + now rewrite <- Heqt0.                         
+    - apply KtransObs; auto. now rewrite Heqt0, Heqt.
+    - apply KtransTau; auto. now rewrite Heqt0, Heqt.
+    - apply KtransRet; auto.
+      + now rewrite Heqt.
+      + now rewrite Heqt0. 
   Qed.
+  
+  (*| This version is more amenable to induction |*)
+  Lemma ktrans_trans: forall t t' w w',
+      ktrans_ (t, w) (t', w') <->
+        (exists l, trans_ l (observe t) (observe t') /\
+                ~ is_done w /\
+                ((l = tau /\ w' = w)
+                 \/ (exists e (x: encode e), l = obs e x /\ w' = Obs e x)
+                 \/ (exists (x: X), l = val x /\ t' ≅ stuck /\ w' = Done x))).
+  Proof.
+    intros; split; intro H.
+    inv H. 
+    - exists (obs e x); split; auto; split; auto.
+      right; left.
+      exists e, x; auto.
+    - exists tau; split; auto. 
+    - exists (val x); rewrite H6; split; auto; split; auto.
+      right; right.
+      exists x; auto.
+    - destruct H as (l & ? & ? & ?).
+      + destruct H1.
+        * destruct H1 as (-> & ->).
+          now apply KtransTau.
+        * destruct H1.
+          -- destruct H1 as (e & x & -> & ->).
+             now apply KtransObs.
+          -- destruct H1 as (x & -> & ? & ->).
+             rewrite H1 in *.
+             apply KtransRet; auto.
+  Qed.  
+
 End CTreeTrans.
 
-(** This import messes up instance resolution for [equ eq] *)
-From CTree Require Import CTree.SBisim.
-
 Ltac ktrans_inv H :=
-  let Heqw := fresh "Heqw" in
+  let Hw := fresh "Heqw" in
   let e := fresh "e" in
   let x := fresh "x" in
   let l := fresh "l" in
   let TR := fresh "TR" in
-  simpl ktrans in H;
+  let Ht := fresh "Heqt" in
   apply ktrans_trans in H as
-      (l & H & [(Hl & Hw) | (e & x & Hl & Hw)]); subst.
+      (l & H & ? & [(Hl & Hw) | [(e & x & Hl & Hw) | (x & Hl & Ht & Hw)]]); subst.
 
 Ltac ktrans_goal :=
-  simpl ktrans; apply ktrans_trans.
+  simpl ktrans; eexists; apply ktrans_trans.
 
 Global Hint Constructors ktrans_: core.
 
@@ -95,22 +122,27 @@ Section CTreeTrans.
   Context {E: Type} `{HE: Encode E}.
   Local Open Scope ctl_scope.
   Notation sbisim := (fun (X: Type) => @sbisim E E HE HE X X eq).
-  
+
   (*| CTree is a kripke automaton with [Sb] equivalence |*)
-  #[refine] Global Instance ctree_kripke : Kripke (ctree E) sbisim (Bar E) :=
-    {| ktrans X := ktrans_ (X:=X) |}.
-  Proof.
-    - apply Monad_ctree.
-    - intros.
-      ktrans_inv H0.
-      + destruct (SBisim.sbisim_trans (X:=X) _ _ _ tau eq H H0)
-          as (l & c1' & ? & <- & ?).
-        exists c1'; split; [econstructor|]; auto.      
-      + destruct (SBisim.sbisim_trans (X:=X) _ _ _ (obs e x) eq H H0)
-          as (l & c1' & ? & <- & ?).
-        exists c1'; split; [econstructor|]; auto.
-    - intros.
-      ktrans_inv H; eexists; reflexivity.      
+  Global Program Instance ctree_kripke : Kripke (ctree E) sbisim E :=
+    {| ktrans X m m' := ktrans_ (X:=X) m m' |}.
+  Next Obligation.
+    ktrans_inv H0;
+      destruct (SBisim.sbisim_trans (X:=X) _ _ _ _ eq H H0)
+      as (l & c1' & ? & <- & ?).
+    + exists c1'; split; [apply KtransTau|]; auto.      
+    + exists c1'; split; [apply KtransObs|]; auto.
+    + exists c1'; split; auto.
+      pose proof trans_val_inv H2.
+      rewrite <- H4 in H2.
+      now apply KtransRet. 
+  Defined.
+  Next Obligation.
+    ktrans_inv H; auto with ctl.
+  Defined.
+  Next Obligation.
+    intros (t' & w' & TR).
+    ktrans_inv TR; contradiction.
   Defined.
 
   (*| Lemmas that depend on structure of [ctrees] |*)
@@ -119,34 +151,41 @@ Section CTreeTrans.
         (exists (i: fin' n), (k i, w) ↦ (t', w')).
   Proof.
     split; intro H.
-    - ktrans_inv H; apply trans_brD_inv in H as (n' & ?); exists n'; ktrans_goal.
-      + exists tau; split; [assumption|]; left; auto.
-      + exists (obs e x); split; [assumption|]; right; eauto. 
-    - destruct H as (n' & H); ktrans_inv H; ktrans_goal.
-      + exists tau; split.
+    - ktrans_inv H; apply trans_brD_inv in H as (n' & ?); exists n';
+        apply ktrans_trans; eexists.
+      + split; [eassumption|split]; auto. 
+      + split; [eassumption|split]; auto.
+        right; left; eauto.
+      + split; [eassumption|split]; auto.
+        right; right; eauto.
+    - destruct H as (n' & H); ktrans_inv H; apply ktrans_trans; eexists.
+      + split; [|split].
         * econstructor; eassumption.
+        * assumption.
         * left; split; reflexivity. 
-      + exists (obs e x); split.
+      + split; [|split].
         * econstructor; eassumption.
-        * right; exists e, x; split; reflexivity. 
+        * assumption.
+        * right; left; exists e, x; split; reflexivity.
+      + split; [|split].
+        * econstructor; eassumption.
+        * assumption.
+        * right; right; exists x; split; auto. 
   Qed.
 
-  Lemma ktrans_brS {X}: forall n (t: ctree E X)
-                          (k: fin' n -> ctree E X) w w',
+  Lemma ktrans_brS {X}: forall n (t: ctree E X) (k: fin' n -> ctree E X) w w',
       (BrS n k, w) ↦ (t, w') <->
-        (exists (i: fin' n), t ≅ k i /\ w = w').
+        (exists (i: fin' n), t ≅ k i /\ w = w' /\ ~ is_done w).
   Proof.
     split; intro H.
     - ktrans_inv H; apply trans_brS_inv in H as (n' & ? & ?);
-        exists n'; subst; inv H0; auto.
-    - destruct H as (n' & H & ->).
-      ktrans_goal.
-      exists tau; split; econstructor; [|auto].      
-      (* HACK *)
-      Set Typeclasses Filtered Unification.
-      symmetry.
-      Unset Typeclasses Filtered Unification.
-      apply H.
+        exists n'; subst; inv H1; auto.
+    - destruct H as (n' & -> & -> & ?).
+      apply ktrans_trans; exists tau.
+      split; econstructor.
+      * reflexivity.
+      * auto.
+      * now left.
   Qed.
   
   Lemma ktrans_guard {X}: forall (t t': ctree E X) s s',
@@ -158,326 +197,128 @@ Section CTreeTrans.
   Qed.
 
   Lemma ktrans_ret {X}: forall (t: ctree E X) s s' x,
-      (Ret x, s) ↦ (t, s') -> False.
+      (Ret x, s) ↦ (t, s') <-> (s' = Done x /\ t ≅ stuck /\ ~ is_done s).
   Proof.
-    intros.
-    ktrans_inv H; inv H.
+    intros; split; intros.
+    - ktrans_inv H; dependent destruction H; auto.
+    - destruct H as (-> & -> & ?). 
+      apply KtransRet; etrans.
   Qed.
 
-  Lemma ktrans_vis {X}: forall (t: ctree E X) s s' e (k: encode e -> ctree E X),
-    (Vis e k, s) ↦ (t, s') <->
-      (exists (x: encode e), k x ≅ t /\ s' = Some (Obs e x)).
+  Lemma ktrans_vis {X}: forall (t: ctree E X) (s s': World E) (e: E) (k: encode e -> ctree E X),
+      ktrans_ (Vis e k, s) (t, s') <->
+      (exists (x: encode e), s' = Obs e x /\ k x ≅ t /\ ~ is_done s).
   Proof.
     intros; split; intro TR.
     - ktrans_inv TR.
       + inv TR.
       + cbn in TR.
-        unfold trans in TR.
         dependent induction TR.        
-        exists x0; split. 
+        exists x0; split; [reflexivity|split].
         * step; step in H; cbn in *; rewrite <- x; auto.
-        * reflexivity.
-    - destruct TR as (? & ? & ->).
-      ktrans_goal.
-      exists (obs e x); split; [econstructor|right]; eauto.
-  Qed.
-
-  Lemma ktrans_bind_inv_strong: forall {X Y} w w' (t: ctree E Y) (u: ctree E X) (k: Y -> ctree E X),
-      (x <- t ;; k x, w) ↦ (u, w') ->
-      (exists t', (t, w) ↦ (t', w') /\ u ≅ x <- t' ;; k x) \/
-        (exists x, only_ret t x /\ (k x, w) ↦ (u, w')).
-  Proof.
-    intros * TR.
-    apply ktrans_trans in TR as (l & TR & [(-> & ->) | ?]).
-    - destruct (trans_bind_inv _ _ TR) as
-        [(Hv & t' & TR' & Heq) | (x' & TRv & TR')].
-      + left; exists t'; split; cbn; auto.
-      + admit.
-  Admitted.
-  
-  Lemma ktrans_bind_inv: forall {X Y} w w' (t: ctree E Y) (u: ctree E X) (k: Y -> ctree E X),
-      (x <- t ;; k x, w) ↦ (u, w') ->
-      (exists t', (t, w) ↦ (t', w') /\ u ≅ x <- t' ;; k x) \/
-        (exists x, may_ret t x /\ (k x, w) ↦ (u, w')).
-  Proof.
-    intros * TR.
-    ktrans_inv TR; destruct (trans_bind_inv _ _ TR) as
-      [(Hv & t' & TR' & Heq) | (x' & TRv & TR')].
-    + left; exists t'; split; cbn; auto.
-    + right; exists x'; split; cbn; auto.
-    + left; exists t'; split; cbn; auto.
-    + right; exists x'; split; cbn; auto.
+        * assumption.
+      + inv TR.
+    - destruct TR as (? & -> & <- & ?).
+      apply ktrans_trans; exists (obs e x).
+      split; [econstructor|split]; auto.
+      right; left; eauto.
   Qed.
 
   Lemma ktrans_bind_l: forall {X Y} w w' (t t': ctree E Y) (k: Y -> ctree E X),
-      (t, w) ↦ (t', w') ->
-      (x <- t ;; k x, w) ↦ (x <- t' ;; k x, w').
+      ktrans_ (t, w) (t', w') ->
+      ~ is_done w' ->
+      ktrans_ (x <- t ;; k x, w) (x <- t' ;; k x, w').
   Proof.
     intros.
     ktrans_inv H; apply ktrans_trans.    
     - exists tau; split. (* BrS *)
-      + apply trans_bind_l.
-        * intro Hcontra.
-          inversion Hcontra.
-        * apply H. 
-      + left; auto. 
+      + apply trans_bind_l; auto.
+        intro Hcontra; inv Hcontra.
+      + split; auto.
     - exists (obs e x); split. (* Vis *)
-      + apply trans_bind_l.
-        * intro Hcontra.
-          inversion Hcontra.
-        * apply H. 
-      + right; eauto.
+      + apply trans_bind_l; auto.
+        intro Hcontra; inv Hcontra.
+      + split; try assumption.
+        right; eauto.
+    - exfalso.
+      apply H0; econstructor.
   Qed.
 
-  Lemma ktrans_bind_r: forall {X Y} w w' (t: ctree E Y) (u: ctree E X) (k: Y -> ctree E X) (x: Y),
-      may_ret t x ->
-      (k x, w) ↦ (u, w') ->
-      (x <- t ;; k x, w) ↦ (u, w').
+  Lemma ktrans_bind_r{X Y}: forall w w' (t: ctree E Y) (u: ctree E X)
+                              (k: Y -> ctree E X) (x: Y),
+      ktrans_ (t, w) (stuck, Done x) ->
+      ktrans_ (k x, w) (u, w') ->
+      ktrans_ (x <- t ;; k x, w) (u, w').
   Proof.
     intros.
-    ktrans_inv H0; apply ktrans_trans.
-    - exists tau; split.
-      + apply trans_bind_r with x; eauto.
-      + left; auto.
-    - exists (obs e x0); split.
-      + apply trans_bind_r with x; eauto.
-      + right; eauto.
+    ktrans_inv H.
+    - exfalso; apply H1; econstructor.
+    - inv Heqw.
+    - inv Heqw; invert.
+      ktrans_inv H0; apply ktrans_trans.
+      + exists tau; split.
+        * apply trans_bind_r with x0; etrans. 
+        * split; auto.
+      + exists (obs e x); split.
+        * apply trans_bind_r with x0; etrans.
+        * split; [auto|].
+          right; left; eauto.
+      + exists (val x); split.
+        * apply trans_bind_r with x0; etrans.
+        * split; [auto|].
+          right; right; eauto.
+  Qed.
+  
+  Lemma ktrans_bind_inv{X Y}:
+    forall w w' (t: ctree E Y) (u: ctree E X) (k: Y -> ctree E X),
+      ktrans_ (x <- t ;; k x, w) (u, w') ->
+      ( ~ is_done w' /\ exists t', ktrans_ (t, w) (t', w') /\ u ≅ x <- t' ;; k x) \/
+        ( exists x, ktrans_ (t, w) (stuck, Done x) /\ ktrans_ (k x, w) (u, w')).
+  Proof.
+    intros * TR.
+    ktrans_inv TR; destruct (trans_bind_inv _ _ TR) as
+      [(Hv & t' & TR' & Heq) | (x' & TRv & TR')].
+    + left; split; auto.
+      exists t'; split; cbn; auto.
+    + right; exists x'; split; cbn; auto.
+    + left; split; auto.
+      * intros Hcontra; inv Hcontra.
+      * exists t'; split; cbn; auto.
+    + right; exists x'; split; cbn; auto.
+    + exfalso; apply Hv; econstructor.
+    + right.
+      exists x'; split; apply ktrans_trans.
+      * exists (val x'); split; auto; split; auto.
+        right; right; eauto.
+      * exists (val x); split; auto; split; auto.
+        right; right; eauto.
   Qed.
 
-  Lemma ktrans_bind_inv_l: forall {X Y} w w' (t: ctree E Y) (u: ctree E X) (k: Y -> ctree E X),
-      (x <- t ;; k x, w) ↦ (u, w') ->
-      ~ (exists (x: Y), may_ret t x) ->
-      (exists t', (t, w) ↦ (t', w') /\ u ≅ x <- t' ;; k x).
+  Lemma ktrans_bind_inv_l{X Y}: forall w w' (t: ctree E Y) (u: ctree E X)
+                                  (k: Y -> ctree E X),
+      ktrans_ (x <- t ;; k x, w) (u, w') ->      
+      (exists t' w'', ktrans_ (t, w) (t', w'')).
   Proof.
     intros.
     apply ktrans_bind_inv in H.
-    destruct H as [(? & ?) | (x0 & Hret & Hcont)]; eauto.
-    exfalso.
-    apply H0.
-    now exists x0.
+    destruct H as [(? & ? & ? & ?) | (x0 & Hret & Hcont)]; eauto.
   Qed.
 
-  Lemma ktrans_bind_inv_noret{X Y}: forall w w' (t: ctree E X) (u u': ctree E Y),
-      (t ;; u, w) ↦ (u', w') ->
-      (exists t', (t, w) ↦ (t', w') /\ u' ≅ t' ;; u) \/
-        (exists (x: X), may_ret t x /\ (u, w) ↦ (u', w')).
-  Proof.
-    intros.
-    apply ktrans_bind_inv in H.
-    destruct H as [(? & ?) | (x0 & Hret & Hcont)]; eauto.
-  Qed.
-
-  Lemma can_step_bind_inv_l{X Y}: forall (t: ctree E Y) (k: Y -> ctree E X) w,
-      can_step (x <- t ;; k x, w) ->
-      ~ (exists x, may_ret t x) ->
-      can_step (t, w).
-  Proof.
-    intros.
-    unfold can_step. 
-    destruct H as (t' & w' & TR).
-    destruct (ktrans_bind_inv_l _ _ _ _ _ TR); auto.
-    destruct H.
-    now (exists x, w').
-  Qed.
-  
-  (*| DELETE this weak version after completing the proof [ktrans_bind_inv_strong] |*)
-  Lemma can_step_bind_inv{X Y}: forall (t: ctree E Y) (k: Y -> ctree E X) w,
-      can_step (x <- t ;; k x, w) ->
-      can_step (t, w) \/ (exists x, may_ret t x /\ can_step (k x, w)).
-  Proof.    
-    intros.    
-    destruct H as (t' & w' & TR).    
-    destruct (ktrans_bind_inv _ _ _ _ _ TR) as [(t0 & ? & ?) | (x0 & ?)].
-    - left.
-      now (exists t0, w').
-    - destruct H as (Hret & TR').
-      right.
-      exists x0; split; eauto.
-  Qed.
-  
-  (*| Keep this strong version |*)
-  Lemma can_step_bind_inv_strong{X Y}: forall (t: ctree E Y) (k: Y -> ctree E X) w,
-      can_step (x <- t ;; k x, w) ->
-      can_step (t, w) \/ (exists x, only_ret t x /\ can_step (k x, w)).
-  Proof.    
-    intros.    
-    destruct H as (t' & w' & TR).    
-    destruct (ktrans_bind_inv_strong _ _ _ _ _ TR)
-      as [(t0 & ? & ?) | (x0 & ?)].
-    - left.
-      now (exists t0, w').
-    - destruct H as (Hret & TR').
-      right.
-      exists x0; split; eauto.
-  Qed.
-
-  (*| If [t] steps then [t >>= k] steps |*)
-  Lemma can_step_bind_l{X Y}: forall (t: ctree E Y) (k: Y -> ctree E X) w,
-      can_step (t, w) ->
-      can_step (x <- t;; k x, w).
-  Proof.
-    intros.
-    destruct H as (t' & w' & TR).
-    exists (x <- t';; k x), w'.
-    now apply ktrans_bind_l.
-  Qed.
-  Hint Resolve can_step_bind_l: ctree.
-  
-  (*| If there exists a [t -(val x)-> t'] transition,
-      and [k x] can step then [t >>= k] can step |*)
-  Lemma can_step_bind_r{X Y}: forall (t: ctree E Y) (k: Y -> ctree E X) w x,
-      may_ret t x ->
-      can_step (k x, w) ->
-      can_step (x <- t;; k x, w).
-  Proof.
-    intros.
-    destruct H0 as (t' & w' & TR).
-    exists t', w'.
-    apply ktrans_bind_r with x; auto.
-  Qed.
-  Hint Resolve can_step_bind_r: ctree.
-  
-    (*| [can_step] and [only_ret] are mutually exclusive |*)
-  Lemma can_step_only_ret{X}: forall (t: ctree E X) w,
-      can_step (t, w) ->  ~ (exists x, only_ret t x).
-  Proof.
-    intros * (? & ? & ?) (? & Hcontra).
-    unfold only_ret in Hcontra.
-    apply ktrans_trans in H as (l & TR & ?).
-    remember (observe t) as T.
-    generalize dependent t.
-    generalize dependent H.
-    generalize dependent TR.
-    revert l x0 x w.
-    induction Hcontra; intros.
-    - (* OnlyBrD *)
-      apply trans_brD_inv in TR as (i & ?).
-      eapply H0; eauto.
-    - (* OnlyRet *)
-      apply trans_ret_inv in TR as (? & ->).
-      destruct H as [(? & ?) | (? & ? & ? & ? )];
-        inversion H.
-  Qed.
-  Hint Resolve can_step_only_ret: ctree.
-  
-  Lemma only_ret_can_step{X}: forall (t: ctree E X) x,
-      only_ret t x -> ~ (exists w, can_step (t, w)).
-  Proof.
-    intros.
-    unfold only_ret in H.
-    unfold can_step.
-    setoid_rewrite ktrans_trans.
-    dependent induction H; rewrite <- x.
-    - (* OnlyBrD *)
-      intros (e & t' & e' & l & TR & Hl).
-      apply trans_brD_inv in TR as (i & ?).
-      eapply H0 with (i:=i).
-      + reflexivity.
-      + do 4 eexists; split; eauto.
-    - (* OnlyRet *)
-      intros (e & t' & e' & l & TR & Hl).
-      apply trans_ret_inv in TR as (? & ->).
-      destruct Hl as [(Hcontra & ->)|(? & ? & Hcontra & ?)];
-        inversion Hcontra.
-  Qed.
-  Hint Resolve only_ret_can_step: ctree.
-  
-  (*| [ktrans] with [bind] of [only_ret] means [k x] must step |*)
-  Lemma ktrans_bind_inv_r_strong{X Y}: forall w w' (t: ctree E Y)
-                                (u: ctree E X) (k: Y -> ctree E X) r,
-    (x <- t;; k x, w) ↦ (u, w') ->
-    only_ret t r ->
-    (k r, w) ↦ (u, w').
-  Proof.
-    intros.
-    apply ktrans_bind_inv_strong in H as [(? & ? & Heq) | (x & ? & H')].
-    - apply only_ret_can_step in H0.
-      exfalso.
-      apply H0.
-      exists w; eauto.
-    - pose proof (only_ret_det _ _ _ H H0); subst.
-      apply H'.
-  Qed.
-  Hint Resolve ktrans_bind_inv_r_strong: ctree.
-
-  Lemma ktrans_bind_inv_l_strong{X Y}: forall w w' (t : ctree E Y)
-                                  (u : ctree E X) (k : Y -> ctree E X),
-      (x <- t;; k x, w) ↦ (u, w') ->
-      can_step (t, w) ->
-      exists t' : ctree E Y, (t, w) ↦ (t', w') /\ u ≅ x <- t';; k x.
-  Proof.
-    intros.
-    apply ktrans_bind_inv_strong in H as [(t' & ? & Heq) | (x & ? & H')].
-    - exists t'; auto.
-    - apply only_ret_can_step in H.
-      exfalso.
-      apply H.
-      now (exists w).
-  Qed.
-  Hint Resolve ktrans_bind_inv_l_strong: ctree.
-  
-  Lemma ktrans_bind_r_strong{X Y}: forall w w' (t: ctree E Y)
-                                     (u: ctree E X) (k: Y -> ctree E X) r,
-      (k r, w) ↦ (u, w') ->
-      only_ret t r ->
-      (x <- t;; k x, w) ↦ (u, w').
-  Proof.
-    intros.
-    apply ktrans_trans in H as (l & ? & ?).
-    pose proof (trans_onlyret _ _ H0).
-    unfold only_ret in H0.
-    dependent induction H0; apply ktrans_trans.
-    - exists l; split.
-      now apply trans_bind_r with x0.
-      apply H1.
-    - exists l; split.
-      now apply trans_bind_r with x0.
-      apply H1.
-  Qed.
-  Hint Resolve ktrans_bind_r_strong: ctree.
-
-  Lemma can_step_bind_r_strong{X Y}: forall (t: ctree E Y) (k: Y -> ctree E X) w x,
-      only_ret t x ->
-      can_step (k x, w) ->
-      can_step (x <- t;; k x, w).
-  Proof.
-    intros.
-    destruct H0 as (t' & w' & TR).
-    exists t', w'.
-    apply ktrans_bind_r_strong with x; auto.
-  Qed.
-  Hint Resolve can_step_bind_r: ctree.
-  
-  (*
-  Lemma ktrans_trigger_inv_noret: forall {X} (w w': opt E) (e: E)
-                                 (u: ctree E X) (u': ctree E X),
-      (trigger e ;; u, w) ↦ (u', w') ->
-      exists (x: encode e), u' ≅ u /\ w' = Some (Obs e x).
+  Local Typeclasses Transparent equ.
+  Lemma ktrans_trigger_inv {X}:
+    forall w w' (e: E) (k: encode e -> ctree E X) (u': ctree E X),
+      ktrans_ (x <- trigger e ;; k x, w) (u', w') ->
+      exists (x: encode e), u' ≅ k x /\ w' = Obs e x.
   Proof.    
     intros.
     apply ktrans_bind_inv in H.
-    destruct H as [(t' & ? & ?) | (x0 & Hret & Hcont)].
-    - unfold trigger in H.      
-      apply ktrans_vis in H as (x & ? & ->).
-      unfold resum, resum_ret, ReSum_refl, ReSumRet_refl in *.
-      exists x; split; [|reflexivity].
-      rewrite H0, <- H, bind_ret_l. (** WHY DO THESE REWRITES TAKE SO LONG? *)
-      
-
-      (* TO DEBUG unification
-         ---------------------
-        Set Debug "unification,tactic-unification".
-
-         TRIED BUT DID NOT HELP
-         ----------------------
-        Set Typeclasses Iterative Deepening.
-        Remove Hints Eq.SBisim.equ_sbisim_subrelation: typeclass_instances.
-        Typeclasses eauto := debug 6.       
-       *)
-      Set Typeclasses Filtered Unification.
-      reflexivity.
-      Unset Typeclasses Filtered Unification.
-      - inv Hret.
-  Qed. *)
-  
+    destruct H as [(? & ? & ? & ?) | (x0 & Hret & Hcont)].
+    - unfold trigger in H0.
+      apply ktrans_vis in H0 as (x' & ? & ? & ?).
+      unfold resum, ReSum_refl, resum_ret, ReSumRet_refl in *; subst.
+      exists x'; split; setoid_rewrite <- H2 in H1; rewrite bind_ret_l in H1; auto.
+    - dependent destruction Hret; exfalso; apply H0; auto with ctl.
+      unfold trans in H; dependent destruction H.
+  Qed.
+ 
 End CTreeTrans.
