theories/Utils/Trc.v
@@ -1,0 +1,135 @@
+From Coq Require Import
+  List
+  Basics
+  Relations.Relation_Definitions
+  Classes.Morphisms.
+
+Import ListNotations.
+
+Generalizable All Variables.
+
+(*| Compose setoid relation [R] n-times with itself |*)
+Fixpoint rel_iter {A}(eqA: relation A)`{Equivalence A eqA}(n: nat) (R: relation A): relation A :=
+  match n with
+  | 0%nat => eqA
+  | (S n)%nat => fun a c => exists b, R a b /\ rel_iter eqA n R b c
+  end.
+
+(*| Transitive reflexive closure of [R] |*)
+Definition trc {A}(eqA: relation A)`{Equivalence A eqA} (R: relation A) (a b: A) :=
+  exists n, rel_iter eqA n R a b.
+Arguments trc /.
+
+Global Instance Reflexive_trc {A}(eqA: relation A)`{Equivalence A eqA} R:
+  Reflexive (trc eqA R).
+Proof.
+  red; intros.
+  exists 0; cbn.
+  reflexivity.
+Qed.  
+
+Lemma R_trc {A}(eqA: relation A)`{Equivalence A eqA} (R: relation A): forall (a b c: A),
+    R a b ->
+    trc eqA R b c ->
+    trc eqA R a c.
+Proof.
+  intros.
+  destruct H1.
+  exists (S x); cbn.
+  exists b; split; auto.
+Qed.
+
+(*| Compose setoid relation [R] n-times with itself with labels [X] |*)
+Fixpoint rel_iter_label {X A}(eqA: relation A)`{Equivalence A eqA}(n: nat)(R: X -> A -> A -> Prop):
+  list X -> A -> A -> Prop :=
+  match n with
+  | 0%nat => fun l a b => l = []%list /\ eqA a b 
+  | (S n)%nat => fun l a c => exists h ts b, (l = h::ts) /\ R h a b /\ rel_iter_label eqA n R ts b c
+  end.
+
+Definition trc_label{X A}(eqA: relation A)`{Equivalence A eqA}(R: X -> A -> A -> Prop)(l: list X)(a b: A):=
+  exists n, rel_iter_label eqA n R l a b.
+
+Arguments trc_label /.
+
+Lemma rel_iter_label_len{X A: Type}`{Equivalence A eqA}: forall n R (l: list X) a b,
+    rel_iter_label eqA n R l a b -> length l = n.
+Proof.    
+  induction n; cbn;intros.
+  - destruct H0 as (-> & ?).
+    reflexivity.
+  - destruct H0 as (h &  ts & b' & -> & HR & HRi).
+    cbn.
+    cut (length ts = n).
+    + intros ->; reflexivity.
+    + eapply IHn; eauto.
+Qed.
+
+Global Instance rel_iter_proper {A} {n: nat} (R: relation A) `{Equivalence A eqA}
+  {HP: Proper (eqA ==> eqA ==> iff) R}:
+  Proper (eqA ==> eqA ==> iff) (rel_iter eqA n R).
+Proof.
+  induction n; unfold Proper, respectful; cbn;
+    intros; split; intros; subst.
+  - symmetry in H0.
+    transitivity x; auto.
+    transitivity x0; auto.
+  - transitivity y; auto.
+    transitivity y0; auto.
+    now symmetry.
+  - destruct H2 as (t' & TR & TRi).
+    exists t'; split.
+    + now rewrite <- H0.
+    + now rewrite <- H1.
+  - destruct H2 as (t' & TR & TRi).
+    exists t'; split.
+    + now rewrite H0.
+    + now rewrite H1.
+Qed.
+
+Global Instance trc_proper {A} (R: relation A) `{Equivalence A eqA}
+  {HP: Proper (eqA ==> eqA ==> iff) R}:
+  Proper (eqA ==> eqA ==> iff) (trc eqA R).
+Proof.
+  unfold Proper, respectful; cbn; intros; split; intros (n & HH); exists n.
+  - now rewrite <- H0, <- H1.
+  - now rewrite H0, H1.
+Qed.
+
+Global Instance rel_iter_label_proper {X A} {n: nat} (R: X -> relation A) `{Equivalence A eqA}
+  {HP: Proper (eq ==> eqA ==> eqA ==> iff) R}:
+  Proper (eq ==> eqA ==> eqA ==> iff) (rel_iter_label eqA n R).
+Proof.
+  induction n; unfold Proper, respectful; cbn;
+    intros; split; intros.
+  - destruct H3 as (-> & ?); subst.
+    split; auto.
+    symmetry in H1.
+    transitivity x0; auto.
+    transitivity x1; auto.
+  - destruct H3 as (-> & ?); subst.
+    split; auto.
+    transitivity y0; auto.
+    transitivity y1; auto.
+    now symmetry.
+  - destruct H3 as (h & ts & c & Eql & HR & TRi).
+    subst.
+    exists h, ts, c; split; auto; split.
+    + now rewrite <- H1.
+    + now rewrite <- H2.
+  - destruct H3 as (h & ts & c & Eql & HR & TRi).
+    subst.
+    exists h, ts, c; split; auto; split.
+    + now rewrite H1.
+    + now rewrite H2.
+Qed.
+
+Global Instance trc_label_proper {X A} (R: X -> relation A) `{Equivalence A eqA}
+  {HP: Proper (eq ==> eqA ==> eqA ==> iff) R}:
+  Proper (eq ==> eqA ==> eqA ==> iff) (trc_label eqA R).
+Proof.
+  unfold Proper, respectful; cbn; intros; split; intros (n & HH); exists n;
+    subst.
+  - now rewrite <- H1, <- H2.
+  - now rewrite H1, H2.
+Qed.
